semantics/gramScript.sml
@@ -106,7 +106,7 @@ val cmlG_def = mk_grammar_def ginfo
        |  ^(``{SymbolT s | s ≠ ""}``)
        |  "*" | "=" ;
 
- Eliteral ::= <IntT> |  <CharT> | <StringT> | <WordT> | <FFIT> ;
+ Eliteral ::= <IntT> | <CharT> | <StringT> | <WordT> | <FFIT> ;
 
  Ebase ::= "(" Eseq ")" | Etuple | "(" ")" | FQV | ConstructorName | Eliteral
         | "let" LetDecs "in" Eseq "end" | "[" "]"
@@ -176,6 +176,8 @@ val cmlG_def = mk_grammar_def ginfo
  TopLevelDecs ::= E ";" TopLevelDecs | TopLevelDec NonETopLevelDecs
                |  ";" TopLevelDecs | ;
  NonETopLevelDecs ::= TopLevelDec NonETopLevelDecs | ";" TopLevelDecs | ;
+ REPLCommand ::= <REPLIDT> Ebase ;
+ TopLevel ::= REPLCommand | TopLevelDecs ;
 `;
 
 val _ = type_abbrev("NT", ``:MMLnonT inf``)
